theories/examples/swap_pair.v
@@ -4,18 +4,19 @@ From iris.prelude Require Import options.
 From melocoton Require Import named_props.
 From melocoton.interop Require Import basics basics_resources.
 From melocoton.interop Require Import lang_to_mlang lang_to_mlang_wp.
-From melocoton.interop Require Import linking linking_wp.
 From melocoton.interop Require Import wrappersem wrapper_wp wrapper_wp_utils wrapper_wp_update_laws wrapper_wp_ext_call_laws wrapper_wp_simulation.
-From melocoton.ml_toy_lang Require Import lang melocoton.primitive_laws.
-From melocoton.ml_toy_lang Require notation melocoton.proofmode.
+From melocoton.ml_toy_lang Require Import lang notation melocoton.primitive_laws.
+From melocoton.ml_toy_lang Require melocoton.proofmode.
 From melocoton.c_toy_lang Require Import lang melocoton.primitive_laws.
 From melocoton.c_toy_lang Require notation melocoton.proofmode.
 From melocoton.mlanguage Require weakestpre.
+From melocoton.interop Require Import linking linking_wp.
 Import uPred.
 
-Section C_prog.
 
-Import melocoton.ml_toy_lang.notation melocoton.c_toy_lang.notation melocoton.c_toy_lang.melocoton.proofmode.
+Section C_prog.
+Import melocoton.c_toy_lang.notation melocoton.c_toy_lang.melocoton.proofmode.
+
 
 Context `{!heapGS_C Σ, !invGS_gen hlc Σ, !primitive_laws.heapGS_ML Σ, !wrapperGS Σ}.
 
@@ -31,9 +32,7 @@ Definition swap_pair_code (x : expr) : expr := (
   (call: &"modify" with (Var "np", Val #0, * ("lv" +ₗ #1))) ;;
   (call: &"unregisterroot" with ( Var "lv" +ₗ #0 )) ;;
   (call: &"unregisterroot" with ( Var "lv" +ₗ #1 )) ;;
-  (* (free ("lv", #2)) ;; *) (* TODO: make C proofmode work with multi-free *)
-  (free ("lv" +ₗ #0, #1)) ;;
-  (free ("lv" +ₗ #1, #1)) ;;
+  (free ("lv", #2)) ;;
   "np"
 )%E.
 
@@ -61,6 +60,7 @@ Proof.
   change (Z.to_nat 2) with 2. cbn. iDestruct "H" as "(H1&H2&_)". destruct rr as [rr].
   wp_pures.
 
+  (* readfield 1 *)
   wp_extern. cbn.
   iModIntro. do 5 iRight; iLeft.
   iExists _, _, _, _, _, _, _, _. unfold named. iFrame "HGC".
@@ -69,8 +69,10 @@ Proof.
   do 2 (iSplitR; first done).
   iIntros (v wlv1) "HGC #Helem1". change (Z.to_nat 0) with 0. cbn -[lstore_own_elem].
   iIntros (Heq Hrepr1); injection Heq; intros <-. clear Heq.
+  wp_store.
 
-  wp_store. wp_pures.
+  (* readfield 2 *)
+  wp_pures.
   wp_extern. cbn.
   iModIntro. do 5 iRight; iLeft.
   iExists _, _, _, _, _, _, _, _. unfold named. iFrame "HGC".
@@ -79,8 +81,10 @@ Proof.
   do 2 (iSplitR; first done).
   iIntros (v wlv2) "HGC #Helem2". change (Z.to_nat 1) with 1. cbn -[lstore_own_elem].
   iIntros (Heq Hrepr2); injection Heq; intros <-. clear Heq.
-  
-  wp_store. wp_pures.
+  wp_store.
+
+  (* registerroot 1 *)
+  wp_pures.
   wp_extern. cbn.
   iModIntro. do 2 iRight; iLeft.
   iExists _, _, _, _. unfold named. iFrame "HGC".
@@ -88,6 +92,7 @@ Proof.
   iSplitR; first done.
   iIntros "HGC H1r".
 
+  (* registerroot 2 *)
   wp_pures.
   wp_extern. cbn.
   iModIntro. do 2 iRight; iLeft.
@@ -96,6 +101,7 @@ Proof.
   iSplitR; first done.
   iIntros "HGC H2r".
 
+  (* alloc *)
   wp_pures.
   wp_extern. cbn.
   iModIntro. do 6 iRight.
@@ -104,10 +110,12 @@ Proof.
   iIntros (θ' γnew wnew) "HGC Hnew %Hreprnew".
   wp_pures. change (Z.to_nat 2) with 2. cbn.
 
+  (* load from root *)
   wp_bind (Load _).
   wp_apply (load_from_root with "[HGC H1r]"); first iFrame.
   iIntros (wlv1') "(Hr1&HGC&%Hrepr1')".
 
+  (* modify 1 *)
   wp_pures.
   wp_extern. cbn.
   iModIntro. do 4 iRight; iLeft.
@@ -116,10 +124,12 @@ Proof.
   do 6 (iSplitR; first done).
   iIntros "HGC Hnew1". change (Z.to_nat 1) with 1. cbn.
 
+  (* load from root *)
   wp_pures. wp_bind (Load _).
   wp_apply (load_from_root with "[HGC H2r]"); first iFrame.
   iIntros (wlv2') "(Hr2&HGC&%Hrepr2')".
 
+  (* modify 2 *)
   wp_pures.
   wp_extern. cbn.
   iModIntro. do 4 iRight; iLeft.
@@ -127,6 +137,7 @@ Proof.
   do 6 (iSplitR; first done).
   iIntros "HGC Hnew1". change (Z.to_nat 0) with 0. cbn.
 
+  (* unregisterroot 1 *)
   wp_pures.
   wp_extern. cbn.
   iModIntro. do 3 iRight; iLeft.
@@ -136,6 +147,7 @@ Proof.
   destruct (repr_lval_inj _ _ _ _ Hrepr1' Hrepr1'1). (* ugly subst*) 
   clear Hrepr1'1.
 
+  (* unregisterroot 2 *)
   wp_pures.
   wp_extern. cbn.
   iModIntro. do 3 iRight; iLeft.
@@ -145,10 +157,14 @@ Proof.
   destruct (repr_lval_inj _ _ _ _ Hrepr2' Hrepr2'1). (* ugly subst*)
   clear Hrepr2'1.
 
-  wp_pures. wp_free.
-  wp_pures. wp_free.
+  (* free *)
   wp_pures.
+  iAssert ((Loc rr) ↦∗ [Some wlv1'; Some wlv2'])%I with "[Hr1 Hr2]" as "Hrr".
+  1: cbn; iFrame.
+  wp_free.
 
+  (* Finish, convert points-to *)
+  wp_pures.
   iMod (freeze_to_immut γnew _ θ' with "[$]") as "(HGC&Hnew)".
 
   iModIntro. iExists θ', (Lloc γnew), _.
@@ -180,7 +196,7 @@ End C_prog.
 
 Section ML_prog.
 
-Import melocoton.ml_toy_lang.lang melocoton.ml_toy_lang.notation melocoton.ml_toy_lang.melocoton.proofmode.
+Import melocoton.ml_toy_lang.melocoton.proofmode.
 
 Context `{!heapGS_C Σ, !invGS_gen hlc Σ, !heapGS_ML Σ, !wrapperGS Σ, !linkGS Σ}.
 
@@ -211,28 +227,29 @@ Definition linked_env : prog_environ combined_lang Σ:= {| penv_prog := fmap inl
 
 Lemma is_linkable_swap_pair : is_link_environ swap_pair_env_lifted client_env_lifted linked_env.
 Proof.
-  split.
-  - cbn. rewrite dom_empty_L. set_solver.
-  - cbn. rewrite fmap_empty  map_union_empty. done.
-  - cbn. iIntros (fn F vs Φ E H1) "%H2". done.
-  - cbn. unfold swap_pair_mod.
+  split; cbn.
+  - rewrite dom_empty_L. set_solver.
+  - rewrite fmap_empty  map_union_empty. done.
+  - iIntros (fn F vs Φ E H1) "%H2". done.
+  - unfold swap_pair_mod.
     iIntros (fn F vs Φ E [<- <-]%lookup_singleton_Some).
     iIntros "(%v1&%v2&_&->&HΦ)".
     unfold Wrap.apply_func. iExists _. iSplitR; first done.
     iNext. iIntros "Hbound". iApply (@wp_wand with "[Hbound]").
     1: by iApply swap_pair_wrapped.
     iIntros (v) "(->&Hbound)". iFrame.
-  - cbn. done.
-  - cbn. unfold swap_pair_ml_spec.
+  - done.
+  - unfold swap_pair_ml_spec.
     iIntros (fname vs Φ H1 H2) "(%&%&->&->&_)". unfold swap_pair_mod in H1.
     rewrite lookup_singleton in H1. congruence.
 Qed.
-Import linking_wp.
+
 Notation link_in_state := (link_in_state wrap_lang (lang_to_mlang ML_lang)).
 
 Lemma linked_prog_correct_overall E : 
     link_in_state In2
- -∗ WP LkSE (Link.Expr2 swap_pair_client) @ linked_env; E {{ λ v, ⌜v = (#1,#2,#3)⌝%V ∗ link_in_state Boundary }}.
+ -∗ WP LkSE (Link.Expr2 swap_pair_client) @ linked_env; E 
+    {{ λ v, ⌜v = (#1,#2,#3)⌝%V ∗ link_in_state Boundary }}.
 Proof.
   iIntros "H". iApply (wp_link_run2 with "H []").
   1: apply is_linkable_swap_pair.
@@ -242,6 +259,11 @@ Proof.
 Qed.
 
 End ML_prog.
+
+(*
+Check @linked_prog_correct_overall.
+Print Assumptions linked_prog_correct_overall.
+*)
 
 
 
